feat: new worklist proof, proof of NFA product
feat: classic automaton, clean up reflection

Squash

SSA/Experimental/Bits/AutoStructs/Constructions.lean
@@ -5,32 +5,49 @@ import Mathlib.Data.Fintype.Prod
 import Mathlib.Data.Finset.Powerset
 import SSA.Experimental.Bits.AutoStructs.Basic
 import SSA.Experimental.Bits.AutoStructs.ForLean
+import SSA.Experimental.Bits.AutoStructs.ForMathlib
 import SSA.Experimental.Bits.AutoStructs.FinEnum
 import SSA.Experimental.Bits.AutoStructs.NFA'
+import SSA.Experimental.Bits.AutoStructs.Worklist
 
 section sink
 
 variable {A : Type} [BEq A] [Hashable A] [DecidableEq A] [FinEnum A]
 
-
 def RawCNFA.addSink (m : RawCNFA A) : RawCNFA A := m.createSink.2
--- def RawCNFA.addSink (m : RawCNFA A) : RawCNFA A :=
-  -- let res := (List.range m.stateMax).foldl (init := (none, m)) fun (sink?, m) s =>
-  --   (FinEnum.toList (α := A)).foldl (init := (sink?, m)) fun (sink?, m) a =>
-  --     let stuck := if let some trans := m.trans.get? (s, a) then trans.isEmpty else true
-  --     if !stuck then (sink?, m) else
-  --       let (sink, m) := match sink? with
-  --                       | some s => (s, m)
-  --                       | none => m.createSink
-  --       (some sink, m.addTrans a s sink)
-  -- res.2
 
-def CNFA.addSink (m : CNFA n) : CNFA n := ⟨m.m.addSink, sorry⟩
+def CNFA.addSink (m : CNFA n) : CNFA n := ⟨m.m.addSink, wf_createSink m.wf⟩
 
 lemma addSink_spec (m : CNFA n) (M : NFA' n) :
     m.Sim M →
-    m.addSink.Sim M.complete :=
-  sorry
+    m.addSink.Sim M.complete := by
+  rintro ⟨Ri, hsim⟩
+  let R (s : State) (q : M.complete.σ) :=
+    s = m.m.stateMax ∧ q = .inr () ∨
+      ∃ qᵢ, s ∈ m.m.states ∧ q = .inl qᵢ ∧ Ri s qᵢ
+  use R; constructor
+  · simp [CNFA.addSink, RawCNFA.addSink, NFA'.complete, NFA.complete, R]
+    rintro s; constructor
+    · rintro q hin hRi; exact hsim.accept hRi
+    · rintro rfl hc; apply m.wf.finals_lt at hc; simp_all
+  · simp [CNFA.addSink, RawCNFA.addSink, NFA'.complete, NFA.complete, R]
+    rintro s (rfl | hi); (right; rfl); left
+    have ⟨q, hs, hRi⟩ := hsim.initial₁ hi
+    exact ⟨q, hs, m.wf.initials_lt hi, hRi⟩
+  · simp [CNFA.addSink, RawCNFA.addSink, NFA'.complete, NFA.complete, R]
+    rintro q hq; obtain ⟨s, hi, hRi⟩ := hsim.initial₂ hq
+    use s, .inr hi, m.wf.initials_lt hi, hRi
+  · simp [CNFA.addSink, RawCNFA.addSink, NFA'.complete, NFA.complete, R]
+    rintro s s' a; constructor
+    on_goal 2 => rintro rfl (⟨_, rfl⟩ | hh); rfl; simp_all
+    rintro q hs hRi (⟨rfl, rfl⟩ | ⟨hs1, hs2, htr⟩)
+    · simp at hs
+    · obtain ⟨_, _, _⟩ := hsim.trans_match₁ hRi htr; tauto
+  · simp [CNFA.addSink, RawCNFA.addSink, NFA'.complete, NFA.complete, R]
+    rintro s a q q' hs hRi hst
+    obtain ⟨s', htr, _⟩ := hsim.trans_match₂ hRi hst (by simp) (by simp)
+    have hs' : s' ∈ m.m.states := m.wf.trans_tgt_lt' _ _ _ htr
+    use s'; tauto
 
 def RawCNFA.flipFinals (m : RawCNFA A) : RawCNFA A :=
   let oldFinals := m.finals
@@ -38,43 +55,254 @@ def RawCNFA.flipFinals (m : RawCNFA A) : RawCNFA A :=
     if oldFinals.contains s then fins else fins.insert s
   { m with finals := newFinals }
 
-def CNFA.flipFinals (m : CNFA n) : CNFA n := ⟨m.m.flipFinals, by sorry⟩
+lemma RawCNFA.flipFinal_wf {m : RawCNFA A} (hwf : m.WF) : m.flipFinals.WF := by
+  simp [flipFinals]
+  constructor <;> simp_all
+
+  let motive (fs : Std.HashSet State) := ∀ s ∈ fs, s ∈ m.states
+  suffices h : motive $ List.foldl (fun fins s => if m.finals.contains s = true then fins else fins.insert s) ∅ (List.range m.stateMax) by
+    exact h
+  apply List.foldlRecOn
+  · simp [motive]
+  · simp [motive]
+    rintro _ _ _ _ _ hif
+    split_ifs at hif <;> simp_all
+    rcases hif <;> simp_all [states]
+  · intros; apply hwf.trans_tgt_lt <;> assumption
+
+def CNFA.flipFinals (m : CNFA n) : CNFA n := ⟨m.m.flipFinals, m.m.flipFinal_wf m.wf⟩
 
 end sink
+
+section generic_prod
+
+variable {α} [BEq α] [Hashable α] [LawfulBEq α]
+variable {β} [BEq β] [Hashable β] [LawfulBEq β]
+variable {S₁ : Finset α} {S₂ : Finset β}
+variable {γ} (f : S₁ → S₂ → γ) (hinj : Function.Injective2 f)
+variable {m₁ : Std.HashSet α} (hm₁ : ∀ s₁ ∈ m₁, s₁ ∈ S₁)
+variable {m₂ : Std.HashSet β} (hm₂ : ∀ s₂ ∈ m₂, s₂ ∈ S₂)
+
+-- generalize to push (f s₁ s₂)
+-- generalize lemmas to an initial a
+
+@[inline]
+def product.prodArray' (a : Array γ) :=
+  m₁.attachWith _ hm₁ |>.fold (init := a) fun is s1 =>
+    m₂.attachWith _ hm₂ |>.fold (init := is) fun is s2 =>
+      is.push (f s1 s2)
+
+@[inline]
+def product.prodArray := prodArray' f hm₁ hm₂ (Array.mkEmpty <| m₁.size * m₂.size)
+
+include hinj in
+omit [BEq α] [Hashable α] [LawfulBEq α] in
+lemma product.prodArray_spec_helper
+    (is : Array γ) (hnd : is.toList.Nodup)
+    (s : S₁) (hnew : ∀ s₂, f s s₂ ∉ is):
+  let motive (a : Array γ) (S : Set S₂)  :=
+    a.toList.Nodup ∧
+    (∃ r, a.toList = is.toList ++ r ∧ (∀ z ∈ r, ∃ s₁ s₂, z = f s₁ s₂)) ∧
+    ∀ s1 s2, f s1 s2 ∈ a ↔ s1 ≠ s ∧ f s1 s2 ∈ is ∨ s1 = s ∧ s2 ∈ S
+  let body := m₂.attachWith _ hm₂ |>.fold (init := is) fun is s2 =>
+      is.push (f s s2)
+  motive body (m₂.attachWith _ hm₂).toSet := by
+  rintro motive; simp only
+  apply Std.HashSet.fold_induction
+  · simp only [motive, hnd, true_and]; use ⟨[], by simp⟩; rintro s₁ s₂
+    simp only [ne_eq, Set.mem_empty_iff_false, and_false, or_false, iff_and_self]
+    rintro hin rfl; exact hnew _ hin
+  rintro a s₂ S hnin ih; split_ands
+  · simp; apply List.Nodup.append ih.1 (by simp)
+    simp only [List.disjoint_singleton, Array.mem_toList]
+    rintro hin
+    rcases ih.2.2 _ _ |>.mp hin with hl | hr
+    · simp at hl
+    · simp [hnin] at hr
+  · obtain ⟨_, ⟨r, hr1, hr2⟩, _⟩ := ih; use r ++ [f s s₂]
+    simp only [Array.push_toList, hr1, List.append_assoc, List.mem_append, List.mem_singleton, true_and]
+    rintro z (hz | rfl)
+    · apply hr2 _ hz
+    · tauto
+  · rintro s₁' s₂'
+    simp [Array.mem_push, ih.2, ne_eq, Prod.mk.injEq, Set.union_singleton, Set.mem_insert_iff,
+      Function.Injective2.eq_iff hinj]
+    tauto
+
+include hinj in
+lemma product.prodArray'_spec_full {aᵢ : Array γ} (hnd: aᵢ.toList.Nodup) (hnin : ∀ s₁ s₂, f s₁ s₂ ∉ aᵢ) :
+    (product.prodArray' f hm₁ hm₂ aᵢ).toList.Nodup ∧
+    (∃ r, (product.prodArray' f hm₁ hm₂ aᵢ).toList = aᵢ.toList ++ r ∧ (∀ z ∈ r, ∃ s₁ s₂, z = f s₁ s₂)) ∧
+    ∀ s₁ s₂, f s₁ s₂ ∈ product.prodArray' f hm₁ hm₂ aᵢ ↔ (s₁.val ∈ m₁ ∧ s₂.val ∈ m₂) := by
+  let motive (a : Array γ) (S : Set S₁) :=
+    a.toList.Nodup ∧
+    (∃ r, a.toList = aᵢ.toList ++ r ∧ (∀ z ∈ r, ∃ s₁ s₂, z = f s₁ s₂)) ∧
+     ∀ s1 s2, f s1 s2 ∈ a ↔ s1 ∈ S ∧ s2.val ∈ m₂
+  suffices h : motive (product.prodArray' f hm₁ hm₂ aᵢ) (m₁.attachWith _ hm₁).toSet by
+    rcases h with ⟨hn, hz, hc⟩; use hn; simp_all
+  simp [product.prodArray']
+  apply Std.HashSet.fold_induction
+  · simp [motive, *]
+  rintro a s S hnin ih
+  obtain ⟨hnd, ⟨r, happ, hf⟩, hels⟩ := prodArray_spec_helper f hinj hm₂ a ih.1 s
+    (by rintro hin; simp [ih.2.2, hnin])
+  obtain ⟨r', happ', hf'⟩ := ih.2.1
+  simp only [Set.union_singleton, hnd, hels, ne_eq, ih.2.2, Std.HashSet.mem_toSet, Std.HashSet.mem_attachWith_mem,
+    Set.mem_insert_iff, true_and, motive]; constructor
+  · use (r' ++ r); simp only [happ, happ', List.append_assoc, List.mem_append, true_and]
+    rintro z (hz | hz)
+    · apply hf' _ hz
+    · apply hf _ hz
+  simp only [Subtype.forall, Std.HashSet.mem_attachWith_mem]; rintro s₁ hs₁ s₂ hs₂; constructor
+  · rintro (⟨h1, h2⟩ | ⟨rfl, h⟩) <;> simp [*]
+  · rintro ⟨rfl | h1, h⟩ <;> simp [*]; exact ne_or_eq ⟨s₁, hs₁⟩ s
+
+include hinj in
+lemma product.prodArray'_spec {aᵢ : Array γ} (hnd: aᵢ.toList.Nodup) (hnin : ∀ s₁ s₂, f s₁ s₂ ∉ aᵢ) :
+    ∀ s₁ s₂, f s₁ s₂ ∈ product.prodArray' f hm₁ hm₂ aᵢ ↔ (s₁.val ∈ m₁ ∧ s₂.val ∈ m₂) :=
+  (prodArray'_spec_full _ hinj _ _ hnd hnin).2.2
+
+include hinj in
+lemma product.prodArray_spec_full :
+    (product.prodArray f hm₁ hm₂).toList.Nodup ∧
+    ∀ s₁ s₂, f s₁ s₂ ∈ product.prodArray f hm₁ hm₂ ↔ (s₁.val ∈ m₁ ∧ s₂.val ∈ m₂) := by
+  simp only [prodArray]
+  obtain ⟨h1, _, h2⟩ := prodArray'_spec_full (aᵢ := #[]) f hinj hm₁ hm₂ (by simp) (by simp)
+  simp [h1, h2]
+
+include hinj in
+@[simp]
+lemma product.prodArray_spec :
+    ∀ s₁ s₂, f s₁ s₂ ∈ product.prodArray f hm₁ hm₂ ↔ (s₁.val ∈ m₁ ∧ s₂.val ∈ m₂) :=
+  prodArray_spec_full _ hinj _ _ |>.2
+
+end generic_prod
 
 section product
 
 variable {A : Type} [BEq A] [LawfulBEq A] [Hashable A] [DecidableEq A] [FinEnum A]
 
-omit [LawfulBEq A] in
-lemma RawCNFA.WF.intitials_states (m : RawCNFA A) (hwf : m.WF) : ∀ s ∈ m.initials, s ∈ m.states := by
-  simp_all [RawCNFA.states, hwf]
+def product.inits (m₁ m₂ : CNFA n) :=
+  product.prodArray Prod.mk @m₁.wf.initials_lt @m₂.wf.initials_lt
 
-def product (final? : Bool → Bool → Bool) (m1 m2 : CNFA n) : CNFA n :=
-  worklistRun (m1.m.states × m2.m.states) final inits (by sorry /- looks annoying -/) f
-where final (ss : m1.m.states × m2.m.states) := final? (m1.m.finals.contains ss.1) (m2.m.finals.contains ss.2)
-      inits :=
-       let a := Array.mkEmpty <| m1.m.initials.size * m2.m.initials.size
-       m1.m.initials.attachWith _ m1.wf.intitials_states |>.fold (init := a) fun is s1 =>
-         m2.m.initials.attachWith _ m2.wf.intitials_states |>.fold (init := is) fun is s2 =>
-           is.push (s1, s2)
-      f (ss : m1.m.states × m2.m.states) :=
+def product.inits_nodup : inits m₁ m₂ |>.toList.Nodup := by
+  refine (prodArray_spec_full _ ?_ _ _).1
+  rintro _ _ _ _ ⟨rfl, rfl⟩; trivial
+
+@[simp]
+lemma product.inits_spec :
+    ∀ s₁ s₂, (s₁, s₂) ∈ inits m₁ m₂ ↔ (s₁.val ∈ m₁.m.initials ∧ s₂.val ∈ m₂.m.initials) := by
+  rintro s₁ s₂; simp only [inits]
+  rw [prodArray_spec Prod.mk]
+  rintro _ _ _ _ ⟨rfl, rfl⟩; trivial
+
+def product (final? : Bool → Bool → Bool) (m₁ m₂ : CNFA n) : CNFA n :=
+  worklistRun (m₁.m.states × m₂.m.states) final (product.inits m₁ m₂)
+    (by exact product.inits_nodup) f
+where final (ss : m₁.m.states × m₂.m.states) := final? (ss.1 ∈ m₁.m.finals) (ss.2 ∈ m₂.m.finals)
+      f (ss : m₁.m.states × m₂.m.states) :=
         let (s1, s2) := ss
         (FinEnum.toList (α := BitVec n)).foldl (init := Array.empty) fun as a =>
-          let s1trans := m1.m.trans.getD (s1, a) ∅
-          let s2trans := m2.m.trans.getD (s2, a) ∅
-          s1trans.attachWith _ (m1.wf.trans_tgt_lt' s1 a) |>.fold (init := as) fun as s1' =>
-            s2trans.attachWith _ (m2.wf.trans_tgt_lt' s2 a) |>.fold (init := as) fun as s2' =>
-              as.push (a, (s1', s2'))
-
-
-def CNFA.inter (m1 m2 : CNFA n) : CNFA n := product (fun b1 b2 => b1 && b2) m1 m2
-def CNFA.union (m1 m2 : CNFA n) : CNFA n :=
-  -- FIXME add a sink state to each automata, or modify product
-  product (fun b1 b2 => b1 || b2) m1.addSink m2.addSink
+          product.prodArray' (λ s₁ s₂ ↦ (a, (s₁, s₂))) (m₁.wf.trans_tgt_lt' s1 a) (m₂.wf.trans_tgt_lt' s2 a) as
 
 noncomputable def to_prop (f : Bool → Bool → Bool) (p1 p2 : Prop) : Prop :=
   f (@Decidable.decide p1 (Classical.propDecidable _)) (@Decidable.decide p2 (Classical.propDecidable _))
+
+lemma product.f_spec {m₁ m₂ : CNFA n} {s₁ : m₁.m.states} {s₂ : m₂.m.states} :
+    ∀ a s₁' s₂',
+      (a, (s₁', s₂')) ∈ f m₁ m₂ (s₁, s₂) ↔ s₁'.val ∈ m₁.m.tr s₁ a ∧ s₂'.val ∈ m₂.m.tr s₂ a := by
+  suffices heq :
+      ∀ as a (hnd : as.toList.Nodup) (hnd' : (FinEnum.toList (α := BitVec n)).Nodup)
+       (hnew : ∀ b s₁ s₂, (b, s₁, s₂) ∈ as → b ∉ (FinEnum.toList (α := BitVec n))) s₁' s₂',
+        (a, (s₁', s₂')) ∈
+          ((FinEnum.toList (α := BitVec n)).foldl (init := as) fun as a =>
+          product.prodArray' (λ s₁' s₂' ↦ (a, (s₁', s₂'))) (m₁.wf.trans_tgt_lt' s₁ a) (m₂.wf.trans_tgt_lt' s₂ a) as) ↔
+        (a, (s₁', s₂')) ∈ as ∨ a ∈ (FinEnum.toList (α := BitVec n)) ∧ s₁'.val ∈ m₁.m.tr s₁ a ∧ s₂'.val ∈ m₂.m.tr s₂ a by
+    rintro a s₁' s₂'; rw [f, heq]
+    · simp; rintro h; apply Array.not_mem_empty at h; trivial
+    · exact List.dedup_eq_self.mp rfl
+    · exact FinEnum.nodup_toList
+    · rintro _ _ _ h; apply Array.not_mem_empty at h; trivial
+  induction (FinEnum.toList (α := BitVec n))
+  case nil =>
+    simp only [List.foldl_nil, List.not_mem_nil, false_and, iff_false, Subtype.forall, CNFA.wf]
+    intros _ _ _ _ _ _; tauto
+  case cons a as ih =>
+    rintro bs b hnd hnd' hnew s₁' s₂'
+    obtain ⟨hnd'', ⟨r, hr, hf⟩, hin⟩ := prodArray'_spec_full (fun s₁' s₂' => (a, s₁', s₂'))
+      (by rintro _ _ _ _ ⟨rfl, rfl, rfl⟩; tauto)
+      (m₁.wf.trans_tgt_lt' s₁ a) (m₂.wf.trans_tgt_lt' s₂ a)
+      hnd
+      (by dsimp; rintro s₁ s₂ hin; apply hnew at hin; simp at hin)
+    dsimp
+    have hmem : ∀ b s₁' s₂', b ≠ a → (b, s₁', s₂') ∈ prodArray' (fun s₁' s₂' => (a, s₁', s₂'))
+        (m₁.wf.trans_tgt_lt' s₁ a) (m₂.wf.trans_tgt_lt' s₂ a) bs → (b, s₁', s₂') ∈ bs := by
+      rintro b s₁' s₂' hneq hin
+      rw [Array.mem_def] at hin ⊢; simp only [hr, List.mem_append] at hin
+      rcases hin with hin | hin; assumption
+      obtain ⟨_, _, ⟨rfl, -, -⟩⟩ := hf _ hin; simp at hneq
+    rw [ih] <;> clear ih; rotate_left
+    · apply hnd''
+    · exact (List.nodup_cons.mp hnd').2
+    · rintro b s₁' s₂' hin; by_cases heq : b = a
+      · subst heq; apply List.Nodup.not_mem hnd'
+      · specialize hnew b s₁' s₂' (hmem b s₁' s₂' heq hin); simp at hnew; simp [hnew]
+    by_cases heq :  b = a
+    · subst heq
+      simp [hin]; clear hin; constructor
+      · rintro (⟨h1, h2⟩ | ⟨_, h1, h2⟩) <;> right <;> simp [h1, h2]
+      · rintro (hc | ⟨h1, h2⟩)
+        · apply hnew at hc; simp at hc
+        · left; simp [h1, h2]
+    · simp only [List.mem_cons, heq, false_or]; constructor
+      · rintro (hin | hin)
+        · left; apply hmem _ _ _ heq hin
+        · right; exact hin
+      · rintro (hin | hin)
+        · left; rw [Array.mem_def] at hin ⊢; rw [hr]; simp [hin]
+        · right; exact hin
+
+lemma product.sim {m1 m2 : CNFA n}:
+    m1.Sim M1 → m2.Sim M2 →
+    (nfa (product.inits m1 m2) (final final? m1 m2) (f m1 m2)).Bisim (M1.M.product (to_prop final?) M2.M) := by
+  rintro ⟨R₁, hsim₁⟩ ⟨R₂, hsim₂⟩
+  let R : Rel (m1.m.states × m2.m.states) (M1.σ × M2.σ) :=
+    λ (s₁, s₂) (q₁, q₂) ↦ R₁ s₁ q₁ ∧ R₂ s₂ q₂
+  use R; constructor
+  · rintro ⟨s₁, s₂⟩ ⟨q₁, q₂⟩ ⟨hR₁, hR₂⟩
+    simp [nfa, to_prop, final]
+    rw [←hsim₁.accept hR₁, ←hsim₂.accept hR₂]; congr
+  · constructor
+    · rintro ⟨s₁, s₂⟩ hstart
+      simp [nfa, inits_spec] at hstart; rcases hstart with ⟨h₁, h₂⟩
+      obtain ⟨q₁, hq₁, hR₁⟩ := hsim₁.initial₁ h₁
+      obtain ⟨q₂, hq₂, hR₂⟩ := hsim₂.initial₁ h₂
+      use (q₁, q₂); simp [NFA.product, R, *]
+    · rintro ⟨q₁, q₂⟩ ⟨hst₁, hst₂⟩
+      apply hsim₁.initial₂ at hst₁; obtain ⟨s₁, hi₁, hR₁⟩ := hst₁
+      apply hsim₂.initial₂ at hst₂; obtain ⟨s₂, hi₂, hR₂⟩ := hst₂
+      simp only [nfa, Set.mem_setOf_eq, Prod.exists, inits_spec, exists_and_left, exists_prop]
+      have hin₁ : s₁ ∈ m1.m.states := by apply m1.wf.initials_lt hi₁
+      have hin₂ : s₂ ∈ m2.m.states := by apply m2.wf.initials_lt hi₂
+      use ⟨s₁, hin₁⟩, ⟨s₂, hin₂⟩
+  · rintro ⟨s₁, s₂⟩ ⟨q₁, q₂⟩ a ⟨s₁', s₂'⟩ ⟨hR₁, hR₂⟩ hst
+    simp [nfa, f_spec] at hst; rcases hst with ⟨hst₁, hst₂⟩
+    obtain ⟨q₁', hst₁, hR₁'⟩ := hsim₁.trans_match₁ hR₁ hst₁
+    obtain ⟨q₂', hst₂, hR₂'⟩ := hsim₂.trans_match₁ hR₂ hst₂
+    simp [NFA.product]
+    use q₁', q₂'
+  · rintro ⟨s₁, s₂⟩ ⟨q₁, q₂⟩ a ⟨q₁', q₂'⟩ ⟨hR₁, hR₂⟩ hst
+    simp [NFA.product] at hst; rcases hst with ⟨hst₁, hst₂⟩
+    obtain ⟨s₁', hst₁, hR₁'⟩ := hsim₁.trans_match₂ hR₁ hst₁ (by simp) (by simp)
+    obtain ⟨s₂', hst₂, hR₂'⟩ := hsim₂.trans_match₂ hR₂ hst₂ (by simp) (by simp)
+    have hin₁ : s₁' ∈ m1.m.states := by apply m1.wf.trans_tgt_lt' _ _ _ hst₁;
+    have hin₂ : s₂' ∈ m2.m.states := by apply m2.wf.trans_tgt_lt' _ _ _ hst₂
+    simp only [nfa, Set.mem_setOf_eq, Prod.exists, f_spec, exists_and_left, exists_prop]
+    use ⟨s₁', hin₁⟩, ⟨s₂', hin₂⟩
+
+def CNFA.inter (m1 m2 : CNFA n) : CNFA n := product (fun b1 b2 => b1 && b2) m1 m2
+def CNFA.union (m1 m2 : CNFA n) : CNFA n :=
+  product (fun b1 b2 => b1 || b2) m1.addSink m2.addSink
 
 def CNFA.product_spec (final? : Bool → Bool → Bool) (m1 m2 : CNFA n)
   {M1 : NFA' n} {M2 : NFA' n} :
@@ -128,33 +356,102 @@ variable {A : Type} [BEq A] [LawfulBEq A] [Hashable A] [DecidableEq A] [FinEnum 
 def BitVec.any (b : BitVec w) (f : Fin w → Bool → Bool) :=
   List.finRange w |>.any fun n => f n (b[n])
 
+theorem BitVec.any_iff_exists {bv : BitVec w} :
+    bv.any p ↔ ∃ (i : Fin w), p i (bv.getLsbD i) := by
+  simp [any]; rfl
+
+-- could this become a `where` clause in `determinize`?
+def CNFA.determinize.inits (m : CNFA n) : Array (BitVec m.m.stateMax) :=
+  #[BitVec.ofFn (fun n => n ∈ m.m.initials)]
+
 def CNFA.determinize (m : CNFA n) : CNFA n :=
   worklistRun (BitVec m.m.stateMax)
     (fun ss => ss.any fun n b => b == true && n ∈ m.m.finals)
-    #[BitVec.ofFn (fun n => n ∈ m.m.initials)]
+    (determinize.inits m)
     (by apply List.nodup_singleton)
-    fun (ss : BitVec m.m.stateMax) =>
+    f
+where
+  f := fun (ss : BitVec m.m.stateMax) =>
         (FinEnum.toList (BitVec n)).foldl (init := Array.empty) fun ts a =>
           let ss' := m.m.transSetBV ss a
           ts.push (a, ss')
 
-def NFA'.determinize_spec_nonemp (m : CNFA n)  [Nonempty m.m.states]
-  {M : NFA' n} (hsim : m.Sim M) :
-    m.determinize.Sim M.determinize := by
+private def bv_to_set {m : CNFA n} (bv : BitVec m.m.stateMax) : Set State :=
+  { s | bv.getLsbD s }
+
+lemma transSetBV_spec {m : CNFA n} {ss : BitVec m.m.stateMax} :
+    s' ∈ bv_to_set (m.m.transSetBV ss a) ↔
+      ∃ s ∈ bv_to_set ss, s' ∈ m.m.tr s a :=
+  by sorry
+
+lemma CNFA.determinize.f_spec {m : CNFA n} {a : BitVec n} {sa sa' : BitVec m.m.stateMax} :
+    (a, sa') ∈ (f m sa) ↔ (∀ {s'}, s' ∈ bv_to_set sa' ↔ ∃ s ∈ bv_to_set sa, s' ∈ m.m.tr s a) := by
   sorry
 
-def NFA'.determinize_spec_emp (m : CNFA n) (hemp : m.m.stateMax = 0)
+def CNFA.determinize_spec (m : CNFA n)
   {M : NFA' n} (hsim : m.Sim M) :
     m.determinize.Sim M.determinize := by
-  sorry
+  rcases hsim with ⟨Ri, hsim⟩
+  apply bisim_comp
+  · apply worklistRun_spec
+  let R : Rel (BitVec m.m.stateMax) (Set M.σ) :=
+    λ ss qs ↦ Ri.set_eq (bv_to_set ss) qs
+  use R; constructor
+  · simp [nfa', nfa, NFA'.determinize, NFA.toDFA, BitVec.any_iff_exists]
+    rintro q₁ q₂ hR; constructor
+    · rintro ⟨i, hi, ha⟩
+      obtain ⟨s, hsq₂, hRi⟩ := hR.1 hi
+      use s, hsq₂, hsim.accept hRi |>.mp ha
+    · rintro ⟨s, hs, ha⟩
+      obtain ⟨i, hlsb, hRi⟩ := hR.2 hs
+      have hlt : i < m.m.stateMax :=
+        BitVec.lt_of_getLsbD hlsb
+      use ⟨i, hlt⟩, hlsb, hsim.accept hRi |>.mpr ha
+  · have heq : R (BitVec.ofFn fun n_1 => decide (↑n_1 ∈ m.m.initials)) M.M.start := by
+      constructor
+      · rintro s hi
+        obtain ⟨hlt, hinit⟩ := BitVec.ofFn_getLsbD_true.mp hi
+        simp at hinit
+        exact hsim.initial₁ hinit
+      · rintro q hstart
+        obtain ⟨s, hinit, hRi⟩ := hsim.initial₂ hstart
+        simp [bv_to_set]
+        have hlt : s ∈ m.m.states := by apply m.wf.initials_lt hinit
+        simp [RawCNFA.states] at hlt
+        use s, (by apply BitVec.ofFn_getLsbD_true.mpr; use hlt; simp [hinit])
+    simp only [determinize.inits, nfa', nfa, NFA'.determinize, NFA.toDFA, Array.mem_toArray,
+      List.mem_singleton, Set.setOf_eq_eq_singleton, beq_true, DFA.toNFA_start]
+    constructor
+    · rintro bv hin
+      simp only [Set.mem_singleton_iff] at hin; subst hin
+      use M.M.start; simp [heq]
+    · simp [heq]
+  · simp [nfa', nfa, NFA'.determinize, NFA.toDFA, determinize.f_spec]
+    rintro q₁ q₂ a q₁' hR hq₁'; constructor
+    · rintro s' hs'; obtain ⟨s, hs, htr⟩ := hq₁'.mp hs'
+      obtain ⟨q, hq, hRi⟩ := hR.1 hs
+      obtain ⟨q', hq', hRi'⟩ := hsim.trans_match₁ hRi htr
+      simp_all only [NFA.mem_stepSet]; tauto
+    · simp only [NFA.mem_stepSet]; rintro q' ⟨q, hq, hst⟩
+      obtain ⟨s, hs, hRi⟩ := hR.2 hq
+      obtain ⟨s', hs', hRi'⟩ := hsim.trans_match₂ hRi hst (by simp) (by simp)
+      use s'; simp_all only [Set.top_eq_univ, and_true]; tauto
+  · simp [nfa', nfa, NFA'.determinize, NFA.toDFA, determinize.f_spec]
+    rintro q₁ q₂ a hR
+    use m.m.transSetBV q₁ a
+    constructor
+    · intros s; rw [transSetBV_spec]
+    constructor
+    · intro s' h; obtain ⟨s, hs, htr⟩ := transSetBV_spec.mp h
+      obtain ⟨q, hq, hRi⟩ := hR.1 hs
+      obtain ⟨q', hst, hRi'⟩ := hsim.trans_match₁ hRi htr
+      use q'; simp_all only [Set.top_eq_univ, and_true, NFA.mem_stepSet]; use q
+    · simp [NFA.mem_stepSet]
+      rintro q' q hq hst
+      obtain ⟨s, hs, hRi⟩ := hR.2 hq
+      obtain ⟨s', htr, hRi'⟩ := hsim.trans_match₂ hRi hst (by simp) (by simp)
+      use s'; simp_all [transSetBV_spec]; tauto
 
-def NFA'.determinize_spec (m : CNFA n)
-  {M : NFA' n} (hsim : m.Sim M) :
-    m.determinize.Sim M.determinize := by
-  rcases heq : m.m.stateMax
-  · apply NFA'.determinize_spec_emp <;> simp_all
-  · have _ : Nonempty m.m.states := by use 0; simp_all [RawCNFA.states]
-    apply NFA'.determinize_spec_nonemp; simp_all
 
 def CNFA.neg (m : CNFA n) : CNFA n := m.determinize.flipFinals
 
@@ -260,7 +557,7 @@ def CNFA.lift_spec (m : CNFA n1) (f : Fin n1 → Fin n2) {M : NFA' n1} :
 -- Morally, n1 >= n2
 def RawCNFA.proj (m1: RawCNFA (BitVec n1)) (f : Fin n2 → Fin n1) : RawCNFA (BitVec n2) :=
   let m2 : RawCNFA (BitVec n2) := { m1 with trans := Std.HashMap.empty }
-  m1.trans.keys.foldl (init := m2) fun m2 (s, bv) =>
+  m1.trans.keysArray.foldl (init := m2) fun m2 (s, bv) =>
     let trans := m1.trans.getD (s, bv) ∅
     let bv' := bv.transport f
     let oldtrans := m2.trans.getD (s, bv') ∅
